more

Weidenbach_Book/IsaSAT_CDCL.thy
@@ -4,17 +4,6 @@ theory IsaSAT_CDCL
 begin
 
 paragraph \<open>Combining Together: the Other Rules\<close>
-
-definition count_decided_st_heur :: \<open>_ \<Rightarrow> _\<close> where
-  \<open>count_decided_st_heur = (\<lambda>((_,_,_,_,n, _), _). n)\<close>
-
-lemma count_decided_st_heur[sepref_fr_rules]:
-  \<open>(return o count_decided_st_heur, RETURN o count_decided_st_heur) \<in>
-      isasat_unbounded_assn\<^sup>k \<rightarrow>\<^sub>a uint32_nat_assn\<close>
-  \<open>(return o count_decided_st_heur, RETURN o count_decided_st_heur) \<in>
-      isasat_bounded_assn\<^sup>k \<rightarrow>\<^sub>a uint32_nat_assn\<close>
-  unfolding count_decided_st_heur_def isasat_bounded_assn_def isasat_unbounded_assn_def
-  by (sepref_to_hoare; sep_auto)+
   
 definition cdcl_twl_o_prog_wl_D_heur
  :: \<open>twl_st_wl_heur \<Rightarrow> (bool \<times> twl_st_wl_heur) nres\<close>
